PSK lax type checks with hyperstacks

src/tls/PSK.fst
@@ -2,6 +2,7 @@ module PSK
 
 open FStar.Heap
 open FStar.HyperHeap
+open FStar.HyperStack
 
 open Platform.Bytes
 open Platform.Error
@@ -11,6 +12,7 @@ open TLSConstants
 module MM = MonotoneMap
 module MR = FStar.Monotonic.RRef
 module HH = FStar.HyperHeap
+module HS = FStar.HyperStack
 
 // *** PSK ***
 
@@ -61,17 +63,17 @@ private let app_psk_table : MM.t tls_tables_region psk_identifier app_psk_entry 
 let fresh_pskid i h =
   MM.sel (MR.m_sel h app_psk_table) i = None
 
-let registered_app_psk (i:psk_identifier) (h:HH.t) =
+let registered_app_psk (i:psk_identifier) (h:mem) =
   b2t (is_Some (MM.sel (MR.m_sel h app_psk_table) i))
 
-let valid_app_psk (ctx:pskInfo) (i:psk_identifier) (h:HH.t) =
+let valid_app_psk (ctx:pskInfo) (i:psk_identifier) (h:mem) =
   match MM.sel (MR.m_sel h app_psk_table) i with
   | Some (_, c, _) -> b2t (c = ctx)
   | _ -> False
 
 type ex_app_psk = i:psk_identifier{MR.witnessed (registered_app_psk i)}
 
-let fresh_psk psk (h:HH.t) =
+let fresh_psk psk (h:mem) =
   forall i. match MM.sel (MR.m_sel h app_psk_table) i with
        | Some (psk', _, _) -> ~ (Seq.equal psk psk')
        | None -> True
@@ -98,18 +100,27 @@ let rec fresh_psk_id () =
 // "Application PSK" generator (enforces empty session context)
 // Usual caveat of random producing pairwise distinct keys (TODO)
 
+(*
+ * AR: hack. In lax mode, F* cannot prove that in gen_psk, leaked.ref has id = tls_tables_region.
+ * In the hyperheap model, the id in rref is part of the type itself, here it requires Z3 reasoning.
+ * Adding this function below to get around.
+ *)
+private val __temp_ref_to_rref: #a:Type -> r:reference a -> id:HH.rid{r.id = id} -> Tot (rref id a)
+let  __temp_ref_to_rref #a r id = r.ref
+
 let gen_psk (i:psk_identifier) (ctx:pskInfo)
   : ST unit
   (requires (fun h -> fresh_pskid i h))
   (ensures (fun h0 r h1 ->
+    let app_psk_table_as_hsref = MR.as_hsref app_psk_table in
     modifies (Set.singleton tls_tables_region) h0 h1
-    /\ modifies_rref tls_tables_region !{HH.as_ref (MR.as_rref app_psk_table)} h0 h1
+    /\ modifies_rref tls_tables_region !{HH.as_ref app_psk_table_as_hsref.ref} h0.h h1.h
     /\ registered_app_psk i h1))
   =
   MR.m_recall app_psk_table;
   let psk : app_psk i = CoreCrypto.random 32 in
   let leaked = ralloc tls_tables_region false in
-  let add : app_psk_entry i = (psk, ctx, leaked) in
+  let add : app_psk_entry i = (psk, ctx, (__temp_ref_to_rref leaked tls_tables_region)) in
   MM.extend app_psk_table i add
 
 
